theories/L6_PCPS/dead_param_elim_correct.v
@@ -1,6 +1,6 @@
-Require Import L6.cps L6.identifiers L6.ctx L6.set_util L6.state
-        L6.dead_param_elim L6.Ensembles_util L6.tactics L6.map_util
-        L6.hoisting L6.dead_param_elim_util.
+Require Import L6.cps L6.identifiers L6.ctx L6.set_util L6.state L6.alpha_conv
+        L6.dead_param_elim L6.Ensembles_util L6.tactics L6.map_util L6.cps_util
+        L6.hoisting L6.dead_param_elim_util L6.eval L6.algebra L6.logical_relations.
 Require Import compcert.lib.Coqlib Common.compM Common.Pipeline_utils.
 Require Import Coq.Lists.List Coq.MSets.MSets Coq.MSets.MSetRBT Coq.Numbers.BinNums
         Coq.NArith.BinNat Coq.PArith.BinPos Coq.Sets.Ensembles Omega
@@ -14,6 +14,1044 @@ Open Scope monad_scope.
 
 Open Scope ctx_scope.
 Open Scope fun_scope.
+Open Scope alg_scope.
 Close Scope Z_scope.
 
 
+(* DPE as a relation *)
+
+(* S is the set of formal parameters that have been eliminated from the *current* function.
+   That is, whatever is in S, is undefined in the environment when we execute the code. *)
+Inductive Elim_expr (L : live_fun) (find_tag : var -> option fun_tag) :  exp -> exp -> Prop := 
+| Elim_Constr : 
+    forall (x : var) (ys : list var) (ct : ctor_tag) (e : exp) (e' : exp), 
+      Elim_expr L find_tag e e' ->
+      Elim_expr L find_tag (Econstr x ct ys e) (Econstr x ct ys e')
+| Elim_Prim : 
+    forall (x : var) (g : prim) (ys : list var) (e : exp) (e' : exp), 
+      Elim_expr L find_tag e e' ->
+      Elim_expr L find_tag (Eprim x g ys e) (Eprim x g ys e')
+| Elim_Proj : 
+    forall (x : var) (ct : ctor_tag) (n : N) (y : var) (e : exp) (e' : exp), 
+      Elim_expr L find_tag e e' ->
+      Elim_expr L find_tag (Eproj x ct n y e) (Eproj x ct n y e')
+| Elim_Case: 
+    forall (x : var) (ce : list (ctor_tag * exp)) (ce' : list (ctor_tag * exp)),
+      Forall2 (fun p1 p2 => fst p1 = fst p2 /\ Elim_expr L find_tag (snd p1) (snd p2)) ce ce' -> 
+      Elim_expr L find_tag (Ecase x ce) (Ecase x ce')
+| Elim_Halt : 
+    forall (x : var),
+      Elim_expr L find_tag (Ehalt x) (Ehalt x)
+| Elim_App_Unknown :
+    forall (f : var) (ys : list var) (ft : fun_tag),
+      L ! f = None -> 
+      Elim_expr L find_tag (Eapp f ft ys) (Eapp f ft ys)
+| Elim_App_Known :
+    forall (f : var) (ys : list var) (ft ft' : fun_tag) (bs : list bool),
+      L ! f = Some bs ->
+      find_tag f = Some ft' ->
+      Elim_expr L find_tag (Eapp f ft ys) (Eapp f ft' (live_args ys bs))
+| Elim_Letapp_Unknown :
+    forall (x f : var) (ys : list var) (ys' : list var) (ft : fun_tag) (e e' : exp),
+      L ! f = None ->
+      Elim_expr L find_tag e e' ->
+      Elim_expr L find_tag (Eletapp x f ft ys e) (Eletapp x f ft ys e')
+| Elim_Letapp_Known :
+    forall (x f : var) (ys : list var) (ys' : list var) (ft ft' : fun_tag) (e e' : exp) (bs : list bool),
+      L ! f = Some bs ->
+      find_tag f = Some ft' ->            
+      Elim_expr L find_tag e e' ->
+      Elim_expr L find_tag (Eletapp x f ft ys e) (Eletapp x f ft' (live_args ys bs) e').
+
+Inductive Elim_fundefs (L : live_fun) (find_tag : var -> option fun_tag) : fundefs -> fundefs -> Prop := 
+| Elim_nil : 
+  Elim_fundefs L find_tag Fnil Fnil
+| Elim_cons_in_map : 
+    forall (F : fundefs) (F' : fundefs) (e : exp) (e' : exp) (xs : list var) (bs : list bool)
+           (g : var) (ft ft' : fun_tag) (S : Ensemble var), 
+      L ! g = Some bs ->
+      find_tag g = Some ft' ->            
+      Elim_expr L find_tag e e' ->
+      Elim_fundefs L find_tag F F' ->
+      Elim_fundefs L find_tag (Fcons g ft xs e F) (Fcons g ft' (live_args xs bs) e' F')
+| Elim_cons_not_in_map : 
+    forall (F : fundefs) (F' : fundefs) (e : exp) (e' : exp) (xs : list var) (bs : list bool)
+           (g : var) (ft : fun_tag) (S : Ensemble var), 
+      L ! g = None ->  
+      Elim_expr L find_tag e e' ->
+      Elim_fundefs L find_tag F F' ->
+      Elim_fundefs L find_tag (Fcons g ft xs e F) (Fcons g ft xs e' F'). 
+
+
+(* Inductive Dead_fundefs (L : live_fun) : fundefs -> Prop :=  *)
+(* | Known_Fcons_S : *)
+(*     forall f ft xs e B, *)
+(*       Dead S L e -> *)
+(*       Dead_fundefs S L B -> *)
+(*       Dead_fundefs S L (Fcons f ft xs e B) *)
+(* | Known_Fcons : *)
+(*     forall f ft xs e B, *)
+(*       Dead S L e -> *)
+(*       Dead_fundefs S L B -> *)
+(*       Dead_fundefs S L (Fcons f ft xs e B)       *)
+(* | Known_Fnil :  *)
+(*     Dead_fundefs S L Fnil.  *)
+
+
+Lemma Elim_fundefs_exists_Some L find_tag B B' bs f ft xs e :
+  Elim_fundefs L find_tag B B' ->
+  L ! f = Some bs ->
+  fun_in_fundefs B (f, ft, xs, e) ->
+  exists ft' e',
+    find_tag f = Some ft' /\
+    fun_in_fundefs B' (f, ft', live_args xs bs, e') /\
+    Elim_expr L find_tag e e'.
+Proof.
+  intros. induction H.
+  - inv H1.
+  - inv H1.
+    + inv H5. repeat subst_exp. do 2 eexists. split; eauto. split; eauto. now left.
+    + edestruct IHElim_fundefs. eassumption. destructAll.
+      do 2 eexists. split; eauto. split; eauto. now right; eauto.
+  - inv H1.
+    + inv H4. congruence.
+    + edestruct IHElim_fundefs. eassumption. destructAll.
+      do 2 eexists. split; eauto. split; eauto. now right; eauto.
+Qed.
+
+Lemma Elim_fundefs_exists_None L find_tag B B' f ft xs e :
+  Elim_fundefs L find_tag B B' ->
+  L ! f = None ->
+  fun_in_fundefs B (f, ft, xs, e) ->
+  exists e',    
+    fun_in_fundefs B' (f, ft, xs, e') /\
+    Elim_expr L find_tag e e'.
+Proof.
+  intros. induction H.
+  - inv H1.
+  - inv H1.
+    + inv H5. congruence.
+    + edestruct IHElim_fundefs. eassumption. destructAll.
+      eexists. split; eauto. now right; eauto.
+  - inv H1.
+    + inv H4. repeat subst_exp. eexists. split; eauto. now left.
+    + edestruct IHElim_fundefs. eassumption. destructAll.
+      eexists. split; eauto. now right; eauto.
+Qed.
+
+Lemma Elim_fundefs_name_in_fundefs L find_tag B B' :
+  Elim_fundefs L find_tag B B' ->
+  name_in_fundefs B <--> name_in_fundefs B'.
+Proof.
+  intros H. induction H; simpl; sets.
+Qed. 
+
+
+Lemma live_args_NoDup {A} (xs : list A) bs :
+  NoDup xs ->
+  NoDup (live_args xs bs).
+Proof.
+  revert bs. induction xs; intros.
+  - destruct bs; eauto.
+  - destruct bs; eauto.
+    inv H. simpl. destruct b; eauto.
+    econstructor; eauto.
+
+    intros Hc. eapply live_args_subset in Hc. eauto.
+Qed. 
+
+(** Well-scopedness lemmas **)
+
+Lemma Elim_exp_bound_var L find_tag e e' :
+  Elim_expr L find_tag e e' ->
+  bound_var e' \subset bound_var e.
+Proof.
+  revert e'.
+  induction e using exp_ind'; intros e' Helim; inv Helim;
+    try repeat normalize_bound_var; sets.
+
+  inv H2. 
+  + rewrite !bound_var_Ecase_nil at 1. sets.
+  + inv H2. inv H1. destruct y.
+    repeat normalize_bound_var.
+    simpl in *. subst.
+    eapply Included_Union_compat; eauto.
+    eapply IHe0. econstructor; eauto.
+Qed.   
+
+Lemma Elim_fundefs_bound_var L find_tag B B' :
+  Elim_fundefs L find_tag B B' ->
+  bound_var_fundefs B' \subset bound_var_fundefs B.
+Proof.
+  intros Helim; induction Helim; sets; repeat normalize_bound_var.
+  - eapply Included_Union_compat; sets.
+    eapply Included_Union_compat; sets.
+    eapply live_args_subset.
+    eapply Elim_exp_bound_var in H1. sets.
+  - eapply Included_Union_compat; sets.
+    eapply Included_Union_compat; sets.
+    eapply Elim_exp_bound_var in H0. sets.
+Qed.   
+
+Lemma Elim_exp_unique_bindings L find_tag e e' :
+  Elim_expr L find_tag e e' ->
+  unique_bindings e ->
+  unique_bindings e'.
+Proof.
+  revert e'.
+  induction e using exp_ind'; intros e' Helim Hun; inv Helim;
+    inv Hun; try (now econstructor; eauto);
+      try (now econstructor; eauto; intros Hc; eapply H1; eapply Elim_exp_bound_var; eauto).
+  - inv H2. econstructor; eauto.
+  - inv H2. destruct y. inv H1. econstructor; eauto.
+    
+    eapply IHe0. now econstructor; eauto. eassumption.
+
+    eapply Disjoint_Included_l.
+    eapply Elim_exp_bound_var. eassumption.
+    eapply Disjoint_Included_r.
+    eapply Elim_exp_bound_var. econstructor. eassumption.
+    sets.
+Qed. 
+
+
+Lemma Elim_fundefs_unique_bindings L find_tag B B' :
+  Elim_fundefs L find_tag B B' ->
+  unique_bindings_fundefs B ->
+  unique_bindings_fundefs B'.
+Proof.
+  intros Helim Hun; induction Helim; inv Hun; eauto.
+  - econstructor.
+  - econstructor; eauto.
+    + intros Hc; eapply H7; eapply Elim_exp_bound_var; eauto.
+    + intros Hc; eapply H8; eapply Elim_fundefs_bound_var; eauto.
+    + eapply Disjoint_Included.
+      eapply live_args_subset.
+      eapply Elim_exp_bound_var; eauto.
+      sets.
+    + eapply Disjoint_Included.
+      eapply live_args_subset.
+      eapply Elim_fundefs_bound_var; eauto.
+      sets.
+    + eapply Disjoint_Included.
+      eapply Elim_fundefs_bound_var; eauto.
+      eapply Elim_exp_bound_var; eauto.
+      sets.
+    + intros Hc. eapply live_args_subset in Hc. eauto.
+    + eapply live_args_NoDup. eassumption.
+    + eapply Elim_exp_unique_bindings; eauto.
+  - econstructor; eauto.
+    + intros Hc; eapply H6; eapply Elim_exp_bound_var; eauto.
+    + intros Hc; eapply H7; eapply Elim_fundefs_bound_var; eauto.
+    + eapply Disjoint_Included_l.
+      eapply Elim_exp_bound_var; eauto.
+      sets.
+    + eapply Disjoint_Included_l.
+      eapply Elim_fundefs_bound_var; eauto.
+      sets.
+    + eapply Disjoint_Included.
+      eapply Elim_fundefs_bound_var; eauto.
+      eapply Elim_exp_bound_var; eauto.
+      sets.
+    + eapply Elim_exp_unique_bindings; eauto.
+Qed.   
+
+
+Section Correct.
+
+  Context {fuel : Type} {Hfuel : @fuel_resource fuel} {trace : Type} {Htrace : @trace_resource trace}.
+  
+  Variable cenv : ctor_env.
+
+  Context (PL : @PostT fuel trace) (* Local *)
+          (PG : @PostGT fuel trace).  (* Global *)           
+
+  Context (HPost : Post_properties cenv PL PL PG).
+
+
+  Definition fun_inv (L : live_fun) (find_tag  : var -> option fun_tag) k (rho rho' : env) : Prop :=
+    (forall f, f \in Dom_map L -> exists rho1 B1 f1, M.get f rho = Some (Vfun rho1 B1 f1)) /\ 
+    forall f bs vs1 vs2 j ft1 ft2 rho1 rho1' B1 f1 xs1 e1,
+      L ! f = Some bs -> 
+      find_tag f = Some ft2 -> 
+      M.get f rho = Some (Vfun rho1 B1 f1) ->
+      find_def f1 B1 = Some (ft1, xs1, e1) ->
+      Some rho1' = set_lists xs1 vs1 (def_funs B1 B1 rho1 rho1) ->
+      length (live_args xs1 bs) = length vs2 ->
+      
+      exists rho2 rho2' B2 f2 xs2 e2,
+        M.get f rho' = Some (Vfun rho2 B2 f2) /\
+        find_def f2 B2 = Some (ft2, xs2, e2) /\
+        Some rho2' = set_lists xs2 vs2 (def_funs B2 B2 rho2 rho2) /\
+
+        (j < k -> Forall2 (preord_val cenv PG j) (live_args vs1 bs) vs2 ->
+         preord_exp cenv PL PG j (e1, rho1') (e2, rho2')).
+
+
+  
+  (* Lemmas about fun_inv *)
+
+  Lemma fun_inv_set_Disjoint_l L find_tag k x v1 rho1 rho2 :
+    fun_inv L find_tag k rho1 rho2 ->
+    Disjoint _ [set x] (Dom_map L) ->
+    fun_inv L find_tag k (M.set x v1 rho1) rho2.
+  Proof.
+    intros Hinv Hd. split. 
+    { intro; intros.
+      destruct (peq x f).
+      - subst. exfalso. eapply Hd. constructor; eauto.
+      - rewrite !M.gso in *; eauto. eapply Hinv. eauto. }
+    
+    { intro; intros. destruct (peq x f).
+      - subst. exfalso. eapply Hd. constructor; eauto. eexists; eassumption.
+      - rewrite !M.gso in *; eauto. eapply Hinv; eauto. }
+  Qed. 
+
+  Lemma fun_inv_set_Disjoint_r L find_tag k x v1 rho1 rho2 :
+    fun_inv L find_tag k rho1 rho2 ->
+    Disjoint _ [set x] (Dom_map L) ->
+    fun_inv L find_tag k rho1 (M.set x v1 rho2).
+  Proof.
+    intros Hinv Hd. split. 
+    { intro; intros.
+      destruct (peq x f).
+      - subst. exfalso. eapply Hd. constructor; eauto.        
+      - eapply Hinv. eauto. }
+    
+    { intro; intros. destruct (peq x f).
+      - subst. exfalso. eapply Hd. constructor; eauto. eexists; eassumption.
+      - rewrite !M.gso in *; eauto. eapply Hinv; eauto. }
+  Qed. 
+  
+  Lemma fun_inv_set_Disjoint L find_tag k x v1 v2 rho1 rho2 :
+    fun_inv L find_tag k rho1 rho2 ->
+    Disjoint _ [set x] (Dom_map L) ->
+    fun_inv L find_tag k (M.set x v1 rho1) (M.set x v2 rho2).
+  Proof.
+    intros Hinv Hd.
+    eapply fun_inv_set_Disjoint_l; eauto.
+    eapply fun_inv_set_Disjoint_r; eauto.
+  Qed.
+
+
+  Lemma fun_inv_set_lists_Disjoint_l L find_tag k xs vs rho1 rho2 rho1' :
+    fun_inv L find_tag k rho1 rho2 ->
+    Disjoint _ (FromList xs) (Dom_map L) ->
+    set_lists xs vs rho1 = Some rho1' ->
+    fun_inv L find_tag k rho1' rho2.
+  Proof.
+    revert vs rho1 rho2 rho1'; induction xs; simpl; intros vs rho1 rho2 rho1' Hf Hdis Hset. 
+    - destruct vs; congruence.
+    - destruct vs; try congruence.
+      destruct (set_lists xs vs rho1) eqn:Heq. repeat normalize_sets. 
+      inv Hset. 
+      eapply fun_inv_set_Disjoint_l; sets.
+      congruence.
+  Qed. 
+
+
+  Lemma fun_inv_set_lists_Disjoint_r L find_tag k xs vs rho1 rho2 rho2' :
+    fun_inv L find_tag k rho1 rho2 ->
+    Disjoint _ (FromList xs) (Dom_map L) ->
+    set_lists xs vs rho2 = Some rho2' ->
+    fun_inv L find_tag k rho1 rho2'.
+  Proof.
+    revert vs rho1 rho2 rho2'; induction xs; simpl; intros vs rho1 rho2 rho1' Hf Hdis Hset. 
+    - destruct vs; congruence.
+    - destruct vs; try congruence.
+      destruct (set_lists xs vs rho2) eqn:Heq. repeat normalize_sets. 
+      inv Hset. 
+      eapply fun_inv_set_Disjoint_r; sets.
+      congruence.
+  Qed. 
+
+
+
+  Lemma fun_inv_monotonic L find_tag k m rho1 rho2 :
+    fun_inv L find_tag k rho1 rho2 ->
+    m <= k -> 
+    fun_inv L find_tag m rho1 rho2.
+  Proof.
+    intros [Hyp Hinv] Hd. split; eauto. intro; intros. edestruct Hinv; eauto. destructAll.
+    do 6 eexists. repeat split. eassumption. eassumption. eassumption. intros.
+    eapply preord_exp_monotonic. eapply H8; eauto. omega. omega.
+  Qed. 
+
+  Lemma live_args_nil {A} xs :
+    @live_args A xs [] = xs.
+  Proof. destruct xs; eauto. Qed.
+         
+
+  Lemma preord_env_P_get_list_live_args xs (S : var -> Prop) bs k rho1 rho2 vs1 :
+    preord_env_P cenv PG S k rho1 rho2 ->
+    Included var (FromList (live_args xs bs)) S ->
+    get_list xs rho1 = Some vs1 ->
+    exists vs2 : list val,
+      get_list (live_args xs bs) rho2 = Some vs2 /\ Forall2 (preord_val cenv PG k) (live_args vs1 bs) vs2.
+  Proof with now eauto with Ensembles_DB.
+    revert vs1 bs. induction xs; intros vs1 bs Henv Hinc Hget.
+    - inv Hget. destruct bs; eexists; simpl; split; eauto; econstructor.
+    - simpl in *.
+      destruct (M.get a rho1) eqn:Hgeta; try discriminate.
+      destruct (get_list xs rho1) eqn:Hgetl; try discriminate.
+      inv Hget. 
+      destruct bs; simpl in *.
+      + simpl in *. repeat normalize_sets. edestruct Henv. eapply Hinc. now left. eassumption.
+        inv H.
+        edestruct IHxs with (bs := @nil bool); eauto.
+        { destruct xs; simpl; repeat normalize_sets; sets.
+          eapply Included_trans; [| eassumption ]; simpl. sets. }
+        rewrite live_args_nil in H. destructAll.
+        rewrite live_args_nil in H2.
+        
+        eexists. rewrite H, H0. split. reflexivity. econstructor; eauto.
+      + destruct b.
+        * simpl in *. repeat normalize_sets. edestruct Henv. eapply Hinc. now left. eassumption.
+          inv H.
+          edestruct IHxs; eauto.
+          { eapply Included_trans; [| eassumption ]; simpl. sets. }
+          destructAll.
+          eexists. rewrite H, H0. split. reflexivity. econstructor; eauto.
+
+        * simpl in *. repeat normalize_sets. 
+          edestruct IHxs; eauto.
+  Qed.
+
+
+  Lemma live_args_length {A B} xs ys bs :
+    length xs = length ys ->
+    length (@live_args A xs bs) = length (@live_args B ys bs).
+  Proof.
+    revert ys bs. induction xs; intros; eauto.
+    - destruct ys; try (simpl in * ; congruence).
+      destruct bs; reflexivity.
+    - simpl.
+      destruct ys; try (simpl in * ; congruence). inv H.
+      destruct bs. simpl. congruence.
+      destruct b0; simpl; eauto.
+  Qed. 
+
+  
+  Lemma fun_inv_Eletapp L find_tag S k bs x f ft ys e ft' e' rho rho'
+        (Henv : preord_env_P cenv PG (occurs_free (Eletapp x f ft ys e) \\ S \\ Dom_map L) k rho rho')
+        (Hdis1 : Disjoint _ (Dom_map L) (FromList ys))
+        (Hdis2 : Disjoint _ S (FromList (live_args ys bs)))
+        (Hget : L ! f = Some bs)
+        (Htag : find_tag f = Some ft')
+        (Hinv : fun_inv L find_tag k rho rho')
+        (Hexp : (forall (m : nat) (v1 v2 : val),
+                    m < k ->
+                    preord_val cenv PG m v1 v2 -> preord_exp cenv PL PG m (e, M.set x v1 rho) (e', M.set x v2 rho'))) :
+    
+    preord_exp cenv PL PG k (Eletapp x f ft ys e, rho) (Eletapp x f ft' (live_args ys bs) e', rho').
+  Proof.
+    intros v1 c1 t1 Hleq Hstep. inv Hstep.
+    - eexists OOT, c1, zero. split; [| split; eauto ].
+      + econstructor. eassumption.
+      + eapply lt_one in H. 
+        subst. eapply HPost. eapply zero_one_lt. 
+      + simpl; eauto.
+    - inv H. 
+      + edestruct (preord_env_P_get_list_live_args ys) with (bs := bs) as [vs' [Hgetl' Hprevs]]; eauto.
+        eapply Included_Setminus; [| eapply Included_Setminus ]; sets.
+        eapply Disjoint_Included_l. eapply live_args_subset. now sets.
+        eapply Included_trans. eapply live_args_subset. normalize_occurs_free. sets. 
+        
+        rewrite !to_nat_add in Hleq. unfold one in Hleq. rewrite to_nat_one in Hleq. 
+        destruct Hinv as [_ Hinv].
+        
+        edestruct Hinv with (j := k - 1) as (rhoc & rhoc' & B2 & f2 & xs2 & e2 & Hget2 & Hf2 & Hset & Hval).
+        eassumption. eassumption. eassumption. eassumption. now eauto.
+
+        erewrite <- List_util.Forall2_length with (l2 := vs'); [| eassumption ]. eapply live_args_length.
+        eapply set_lists_length_eq. eassumption.
+
+        edestruct Hval. 
+        omega.
+        eapply List_util.Forall2_monotonic; [| eassumption ]. intros.
+        eapply preord_val_monotonic. eassumption. omega.
+        2:{ eassumption. } omega. 
+        destructAll.
+
+        destruct x0; try contradiction.  
+        
+        edestruct Hexp with (m := k - 1 - to_nat cin1) as (v2' & c2' & t2' & Hstep2' & Hpost' & Hval');
+          [  | | | eassumption | ]. simpl in *.
+        omega. simpl in H1. eassumption. omega. 
+
+        exists v2', (x1 <+> c2' <+> (one (Eletapp x f ft' (live_args ys bs) e'))). eexists.
+        split; [| split ]; eauto.
+        * econstructor 2.
+          econstructor; try eassumption. now eauto.
+        * simpl. eapply HPost. eassumption. eassumption. eassumption. eassumption. eassumption.
+          eapply HGPost. eassumption. eassumption.
+          eassumption.
+        * eapply preord_res_monotonic. eassumption.
+          rewrite !to_nat_add. unfold one. rewrite to_nat_one. omega. 
+      + edestruct (preord_env_P_get_list_live_args ys) with (bs := bs) as [vs' [Hgetl' Hprevs]]; eauto.
+        eapply Included_Setminus; [| eapply Included_Setminus ]; sets.
+        eapply Disjoint_Included_l. eapply live_args_subset. now sets.
+        eapply Included_trans. eapply live_args_subset. normalize_occurs_free. sets. 
+        
+        rewrite !to_nat_add in Hleq. unfold one in Hleq. rewrite to_nat_one in Hleq. 
+        destruct Hinv as [_ Hinv]. 
+        edestruct Hinv with (j := k - 1) as (rhoc & rhoc' & B2 & f2 & xs2 & e2 & Hget2 & Hf2 & Hset & Hval).
+        eassumption. eassumption. eassumption. now eauto. now eauto. 
+        erewrite <- List_util.Forall2_length with (l2 := vs'); [| eassumption ]. eapply live_args_length.
+        eapply set_lists_length_eq. eassumption.
+        
+        edestruct Hval. 
+        omega.
+        eapply List_util.Forall2_monotonic; [| eassumption ]. intros.
+        eapply preord_val_monotonic. eassumption. omega.
+        2:{ eassumption. } omega. 
+        destructAll.
+        
+        destruct x0; try contradiction. 
+        
+        exists OOT, (x1 <+> (one (Eletapp x f ft' (live_args ys bs) e'))). eexists.
+        split; [| split ]; eauto.
+        * econstructor 2.
+          econstructor; try eassumption. now eauto.
+        * simpl. eapply HPost. eassumption. eassumption. eassumption. eassumption.
+          eapply HGPost. eassumption. eassumption.
+  Qed. 
+
+
+  Lemma fun_inv_Eapp L find_tag S k bs f ft ys ft' rho rho'
+        (Henv : preord_env_P cenv PG (occurs_free (Eapp f ft ys) \\ S \\ Dom_map L) k rho rho')
+        (Hdis1 : Disjoint _ (Dom_map L) (FromList ys))
+        (Hdis2 : Disjoint _ S (FromList (live_args ys bs)))
+        (Hget : L ! f = Some bs)
+        (Htag : find_tag f = Some ft')
+        (Hinv : fun_inv L find_tag k rho rho') :
+    
+    preord_exp cenv PL PG k (Eapp f ft ys, rho) (Eapp f ft' (live_args ys bs), rho').
+  Proof.
+    intros v1 c1 t1 Hleq Hstep. inv Hstep.
+    - eexists OOT, c1, zero. split; [| split; eauto ].
+      + econstructor. eassumption.
+      + eapply lt_one in H. 
+        subst. eapply HPost. eapply zero_one_lt. 
+      + simpl; eauto.
+    - inv H. edestruct (preord_env_P_get_list_live_args ys) with (bs := bs) as [vs' [Hgetl' Hprevs]]; eauto.
+      eapply Included_Setminus; [| eapply Included_Setminus ]; sets.
+      eapply Disjoint_Included_l. eapply live_args_subset. now sets.
+      eapply Included_trans. eapply live_args_subset. normalize_occurs_free. sets. 
+      
+      rewrite !to_nat_add in Hleq. unfold one in Hleq. rewrite to_nat_one in Hleq. 
+
+      destruct Hinv as [_ Hinv]. 
+      edestruct Hinv with (j := k - 1) as (rhoc & rhoc' & B2 & f2 & xs2 & e2 & Hget2 & Hf2 & Hset & Hval).
+      eassumption. eassumption. eassumption. now eauto. now eauto. 
+      erewrite <- List_util.Forall2_length with (l2 := vs'); [| eassumption ]. eapply live_args_length.
+      eapply set_lists_length_eq. eassumption.
+
+      edestruct Hval. 
+      omega.
+      eapply List_util.Forall2_monotonic; [| eassumption ]. intros.
+      eapply preord_val_monotonic. eassumption. omega.
+      2:{ eassumption. } omega. 
+      destructAll.
+      
+      do 3 eexists.
+      split; [| split ]; eauto.
+      * econstructor 2.
+        econstructor; try eassumption. now eauto.
+      * simpl. eapply HPost; eauto. eapply HGPost. eassumption. eassumption.
+      * eapply preord_res_monotonic. eassumption.
+        rewrite !to_nat_add. unfold one. rewrite to_nat_one. omega. 
+  Qed.
+  
+    
+  Lemma Elim_expr_correct : 
+    forall k e e' L find_tag S rho1 rho2
+           (Hdis1 : Disjoint _ (Dom_map L) (bound_var e :|: occurs_free e))          
+           
+           (Hd : Dead S L e)
+           (Hk : Known_exp (Dom_map L) e)
+           
+           (Hfinv : fun_inv L find_tag k rho1 rho2)
+           
+           (Henv : preord_env_P cenv PG (occurs_free e \\ S \\ Dom_map L) k rho1 rho2)
+
+           (Hbin : binding_in_map (occurs_free e) rho1)
+
+           (Helim : Elim_expr L find_tag e e'),
+      
+      preord_exp cenv PL PG k (e, rho1) (e', rho2).
+  Proof.
+    induction k as [k IHk] using lt_wf_rec1. intros e.
+    revert k IHk; induction e using exp_ind'; intros; inv Helim; inv Hd; inv Hk; try congruence.
+    (* Constr *)
+    - eapply preord_exp_constr_compat.
+      + now eapply HPost.
+      + now eapply HPost.
+      + rewrite <- (map_id l) at 2. eapply Forall2_preord_var_env_map. now eauto. 
+        normalize_occurs_free. sets.
+      + intros. eapply IHk; eauto.
+
+        * eapply Disjoint_Included_r. eapply bound_var_occurs_free_Econstr_Included. eassumption.
+        * eapply fun_inv_set_Disjoint. eapply fun_inv_monotonic. eassumption. omega.
+          repeat normalize_occurs_free_in_ctx. sets.
+        * eapply preord_env_P_extend.
+          eapply preord_env_P_antimon.
+          eapply preord_env_P_monotonic; [| eassumption ]. omega.
+          normalize_occurs_free. sets. rewrite !Setminus_Union_distr, !Setminus_Union. now sets.
+          rewrite preord_val_eq. simpl. split; eauto.
+        * eapply binding_in_map_antimon.
+          eapply Included_Union_Setminus with (s2 := [set v]); tci. eapply binding_in_map_set.
+          eapply binding_in_map_antimon; eauto. normalize_occurs_free. sets.
+
+    - (* Ecase nil *)
+      inv H2.
+      eapply preord_exp_case_nil_compat. now eapply HPost.
+
+    - (* Ecase cons *)
+      inv H2. inv H0. inv H3. destructAll. destruct y. simpl in H; subst.  
+      eapply preord_exp_case_cons_compat_alt.
+      + now eapply HPost.
+      + now eapply HPost.
+      + now eapply HPost.
+      + eapply List_util.Forall2_monotonic; [| eassumption ].
+        intros [? ?] [? ?]. simpl; intros [? ?]; eauto.
+      + intros Heq. destructAll. eapply Henv. 
+        constructor. constructor. normalize_occurs_free. now sets.
+        eassumption.
+        intros Hc. eapply Hfinv in Hc. destructAll. congruence.
+      + intros. eapply IHe; eauto.
+        * intros; eauto. eapply IHk; eauto. omega.
+        * eapply Disjoint_Included_r.
+          eapply bound_var_occurs_free_Ecase_Included. 2:{ eassumption. } now left.
+        * eapply fun_inv_monotonic; eauto. omega. 
+        * eapply preord_env_P_antimon.
+          eapply preord_env_P_monotonic; [| eassumption ]. omega.
+          normalize_occurs_free. sets.
+        * eapply binding_in_map_antimon; [| eassumption ].
+          normalize_occurs_free. sets.
+
+      + eapply IHe0; eauto.
+        * eapply Disjoint_Included_r.
+          eapply bound_var_occurs_free_Ecase_cons_Included. eassumption.
+        * constructor; eauto.
+        * constructor; eauto.
+        * eapply preord_env_P_antimon.
+          eapply preord_env_P_monotonic; [| eassumption ]. omega.
+          normalize_occurs_free. sets.
+        * eapply binding_in_map_antimon; [| eassumption ].
+          normalize_occurs_free. sets.
+        * econstructor. eauto.
+
+    (* Proj *)
+    - eapply preord_exp_proj_compat.
+      + now eapply HPost.
+      + now eapply HPost.
+      + eapply Henv.
+        eapply Included_Setminus with (s1 := [set v0]). now sets.
+        eapply Included_Setminus with (s1 := [set v0]). now sets.
+        normalize_occurs_free. now sets.
+        reflexivity.
+      + intros. eapply IHk; eauto.
+        
+        * eapply Disjoint_Included_r. eapply bound_var_occurs_free_Eproj_Included. eassumption.
+        * eapply fun_inv_set_Disjoint. eapply fun_inv_monotonic; eauto. omega.
+          repeat normalize_occurs_free_in_ctx. sets.
+        * eapply preord_env_P_extend.
+          eapply preord_env_P_antimon.
+          eapply preord_env_P_monotonic; [| eassumption ]. omega.
+          normalize_occurs_free. sets. rewrite !Setminus_Union_distr, !Setminus_Union. now sets.
+          eassumption.
+        * eapply binding_in_map_antimon.
+          eapply Included_Union_Setminus with (s2 := [set v]); tci. eapply binding_in_map_set.
+          eapply binding_in_map_antimon; eauto. normalize_occurs_free. sets.
+
+    - (* Eletapp None *)
+      eapply preord_exp_letapp_compat.
+      + now eapply HPost.
+      + now eapply HPost.
+      + now eapply HPost.
+      + eapply Henv.
+        econstructor.
+        2:{ intros Hin. inv Hin. congruence. }
+        eapply Included_Setminus with (s1 := [set f]). now sets.
+        normalize_occurs_free. now sets.
+        reflexivity.
+      + rewrite <- (map_id ys) at 2. eapply Forall2_preord_var_env_map. now eauto. 
+        normalize_occurs_free. sets.
+      + intros. eapply IHk; eauto.
+        
+        * eapply Disjoint_Included_r. eapply bound_var_occurs_free_Eletapp_Included. eassumption.
+        * eapply fun_inv_set_Disjoint.
+          eapply fun_inv_monotonic; eauto. omega.
+          repeat normalize_occurs_free_in_ctx. sets.
+        * eapply preord_env_P_extend.
+          eapply preord_env_P_antimon.
+          eapply preord_env_P_monotonic; [| eassumption ]. omega.
+          normalize_occurs_free. sets. rewrite !Setminus_Union_distr, !Setminus_Union. now sets.
+          eassumption.
+        * eapply binding_in_map_antimon.
+          eapply Included_Union_Setminus with (s2 := [set x]); tci. eapply binding_in_map_set.
+          eapply binding_in_map_antimon; eauto. normalize_occurs_free. sets.
+          
+    - (* Eletapp Some *)
+      repeat subst_exp. 
+      eapply fun_inv_Eletapp.
+
+      + eassumption.
+      + sets.
+      + sets.
+      + eassumption.
+      + eassumption.
+      + eassumption. 
+      + intros. eapply IHk; eauto.
+        
+        * eapply Disjoint_Included_r. eapply bound_var_occurs_free_Eletapp_Included. eassumption.
+        * eapply fun_inv_set_Disjoint.
+          eapply fun_inv_monotonic; eauto. omega.
+          repeat normalize_occurs_free_in_ctx. sets.
+        * eapply preord_env_P_extend.
+          eapply preord_env_P_antimon.
+          eapply preord_env_P_monotonic; [| eassumption ]. omega.
+          normalize_occurs_free. sets. rewrite !Setminus_Union_distr, !Setminus_Union. now sets.
+          eassumption.
+        * eapply binding_in_map_antimon.
+          eapply Included_Union_Setminus with (s2 := [set x]); tci. eapply binding_in_map_set.
+          eapply binding_in_map_antimon; eauto. normalize_occurs_free. sets.
+
+
+    - (* Eapp None *) 
+      eapply preord_exp_app_compat.
+      + now eapply HPost.
+      + now eapply HPost.
+      + eapply Henv.
+        econstructor.
+        2:{ intros Hin. inv Hin. congruence. }
+        eapply Included_Setminus with (s1 := [set v]). now sets.
+        normalize_occurs_free. now sets.
+        reflexivity.
+      + rewrite <- (map_id l) at 2. eapply Forall2_preord_var_env_map. now eauto. 
+        normalize_occurs_free. sets.
+
+    - (* Eapp Some *)
+      repeat subst_exp. 
+      eapply fun_inv_Eapp. 
+
+      + eassumption.
+      + sets.
+      + sets.
+      + eassumption.
+      + eassumption.
+      + eassumption.
+    - (* Eprim *)
+      eapply preord_exp_prim_compat.
+      + eapply HPost.
+      + rewrite <- (map_id l) at 2. eapply Forall2_preord_var_env_map. now eauto. 
+        normalize_occurs_free. sets. 
+
+    - (* Ehalt *)
+      eapply preord_exp_halt_compat.
+      + eapply HPost.
+      + eapply HPost.
+      + eapply Henv.
+        eapply Included_Setminus with (s1 := [set v]). now sets.
+        eapply Included_Setminus with (s1 := [set v]). now sets.
+        normalize_occurs_free. now sets.
+        reflexivity.
+  Qed.
+
+
+  Lemma Known_fundefs_fun_in_fundefs S B f ft xs e:
+    Known_fundefs S B ->
+    fun_in_fundefs B (f, ft, xs, e) ->
+    Known_exp S e.
+  Proof.
+    intros Hd Hf. induction Hd; inv Hf; eauto.
+    inv H0; eauto.
+  Qed.
+
+  Lemma no_fun_in_fundefs B f ft xs e:
+    no_fun_defs B ->
+    fun_in_fundefs B (f, ft, xs, e) ->
+    no_fun e.
+  Proof.
+    intros Hd Hf. induction Hd; inv Hf; eauto.
+    inv H0; eauto.
+  Qed.
+
+  Lemma dead_args_nil xs :
+    dead_args xs [] = [].
+  Proof.
+    induction xs; eauto.
+  Qed.
+
+  Lemma Dead_empty L e :
+    no_fun e ->
+    Dead (Empty_set var) L e.
+  Proof.
+    induction e using exp_ind'; intros Hnf; inv Hnf; try (now econstructor; sets; eauto).
+    - econstructor; sets.
+      specialize (IHe0 H1). inv IHe0. econstructor; eauto.
+    - destruct (L ! f) eqn:Heq.
+      + eapply Live_LetApp_Known; eauto; sets.
+      + eapply Live_LetApp_Unknown; eauto; sets.
+    - destruct (L ! v) eqn:Heq.
+      + eapply Live_App_Known; eauto; sets.
+      + eapply Live_App_Unknown; eauto; sets.
+  Qed.
+  
+  Lemma preord_env_P_set_lists_live:
+    forall (xs1 : list var) (P : Ensemble var) (rho1 rho2 rho1' rho2' : env)
+           (k : nat) (vs1 vs2 : list val) bs,
+      preord_env_P cenv PG (P \\ FromList xs1) k rho1 rho2 ->
+      Forall2 (preord_val cenv PG k) (live_args vs1 bs) vs2 ->
+      set_lists xs1 vs1 rho1 = Some rho1' ->
+      set_lists (live_args xs1 bs) vs2 rho2 = Some rho2' ->
+      preord_env_P cenv PG (P \\ FromList (dead_args xs1 bs)) k rho1' rho2'.
+  Proof.
+    induction xs1; intros P rho1 rho2 rho1' rho2' k vs1 vs2 bs Henv Hall Hs1 Hs2.
+    + destruct vs1; destruct vs2; destruct bs; simpl in *; try congruence.
+      inv Hs1. inv Hs2. eassumption.
+      inv Hs1. inv Hs2. eassumption.
+    + destruct bs.
+      { rewrite dead_args_nil in *. rewrite live_args_nil in Hall.
+        rewrite live_args_nil in Hs2.
+        normalize_sets.
+        eapply preord_env_P_set_lists_l; eauto.
+        intros. constructor; eauto. inv H0; eauto. } 
+        
+      simpl in *. destruct vs1; try congruence.
+      destruct (set_lists xs1 vs1 rho1) eqn:Hs1'; try congruence.
+      inv Hs1.
+      destruct b.
+      
+      * simpl in *. destruct vs2; try congruence.
+        destruct (set_lists (live_args xs1 bs) vs2 rho2) eqn:Hs2'; try congruence.
+        inv Hs2.
+        
+        inv Hall. eapply preord_env_P_extend; eauto.
+
+        rewrite Setminus_Union. rewrite Union_commut, <- Setminus_Union.
+        eapply IHxs1; eauto.
+        rewrite Setminus_Union. repeat normalize_sets. eassumption.
+
+      * eapply preord_env_P_set_not_in_P_l.
+
+        normalize_sets. rewrite <- Setminus_Union. 
+        eapply IHxs1; eauto.
+        rewrite Setminus_Union. repeat normalize_sets. eassumption.
+
+        normalize_sets. sets.
+  Qed.
+
+
+
+  Lemma Elim_fundefs_correct : 
+    forall k B B' L find_tag rho1 rho2
+           (Hun : unique_bindings_fundefs B)
+           (Hnf : no_fun_defs B)
+           
+           (Hdis1 : Disjoint _ (Dom_map L) (bound_var_fundefs B :|: occurs_free_fundefs B))          
+           (Hdom : Dom_map L \subset name_in_fundefs B)
+           
+           (Hd : live_map_sound B L)
+           (Hk : Known_fundefs (Dom_map L) B)
+           
+           (Hfinv : fun_inv L find_tag k rho1 rho2)
+
+           (Henv : preord_env_P cenv PG (occurs_free_fundefs B \\ Dom_map L) k rho1 rho2)
+
+           (Hbin : binding_in_map (occurs_free_fundefs B) rho1)
+
+           (Helim : Elim_fundefs L find_tag B B'),
+
+      fun_inv L find_tag k (def_funs B B rho1 rho1) (def_funs B' B' rho2 rho2) /\      
+      preord_env_P cenv PG ((name_in_fundefs B :|: occurs_free_fundefs B) \\ Dom_map L) k
+                   (def_funs B B rho1 rho1) (def_funs B' B' rho2 rho2).
+  Proof with now eauto with Ensembles_DB.
+    induction k as [k IHk] using lt_wf_rec1; intros. split.
+
+    - split.
+      + intro; intros. eapply Hdom in H. do 3 eexists. rewrite def_funs_eq. reflexivity. eassumption.
+      + intro; intros.
+        rewrite def_funs_eq in H1. 2:{ eapply Hdom. eexists; eauto. }
+        
+        inv H1. 
+        edestruct Elim_fundefs_exists_Some; try eassumption. eapply find_def_correct. eassumption.
+        destructAll. 
+        
+        rewrite def_funs_eq; eauto.
+        2:{ eapply Elim_fundefs_name_in_fundefs with (B := B1) (B' := B'). eassumption. eapply Hdom. eexists; eauto. }
+        repeat subst_exp.
+
+        edestruct (@set_lists_length3 val) with (xs := live_args xs1 bs) (vs := vs2) (rho := def_funs B' B' rho2 rho2).
+        rewrite <- H4. reflexivity.
+
+        assert (Hand : forall m, m < k ->
+                                 fun_inv L find_tag m (def_funs B1 B1 rho0 rho0) (def_funs B' B' rho2 rho2) /\
+                                 preord_env_P cenv PG
+                                              (name_in_fundefs B1 :|: occurs_free_fundefs B1  \\ Dom_map L) m
+                                              (def_funs B1 B1 rho0 rho0) (def_funs B' B' rho2 rho2)).
+        { intros. eapply IHk; try eassumption.
+          - eapply fun_inv_monotonic. eassumption. omega.
+          - eapply preord_env_P_monotonic; [| eassumption ]. omega. } 
+        
+        do 6 eexists. repeat split.
+        * eapply find_def_complete.
+          eapply unique_bindings_fundefs_unique_functions. 
+          eapply Elim_fundefs_unique_bindings. eassumption. eassumption.
+          eassumption. 
+        * now eauto.
+        * intros.
+          edestruct (Hand j) as [Hinv' Henv']. omega.
+            
+          eapply Elim_expr_correct; try eassumption. 
+          -- eapply Disjoint_Included_r. eapply bound_var_occurs_free_in_fun_Included.
+             eapply find_def_correct. eassumption. eassumption.
+          -- eapply Hd. eapply find_def_correct. eassumption. eassumption.
+          -- eapply Known_fundefs_fun_in_fundefs. eassumption. eapply find_def_correct. eassumption.
+          -- assert (Hin : FromList xs1 \subset bound_var_fundefs B1).
+             { eapply Included_trans; [| eapply fun_in_fundefs_bound_var_fundefs; eapply find_def_correct; eassumption ].
+               sets. } 
+             eapply fun_inv_set_lists_Disjoint_l; eauto; sets.
+             eapply fun_inv_set_lists_Disjoint_r; eauto; sets.
+             eapply Disjoint_Included_l. eapply live_args_subset. sets. 
+          -- rewrite Setminus_Union. rewrite Union_commut, <- Setminus_Union.
+             eapply preord_env_P_set_lists_live; eauto.
+             eapply preord_env_P_antimon. eassumption.
+             rewrite Setminus_Union. rewrite Union_commut, <- Setminus_Union.
+             eapply Included_Setminus_compat. eapply Setminus_Included_Included_Union.
+             eapply Included_trans. eapply occurs_free_in_fun.
+             eapply find_def_correct. eassumption. sets. reflexivity.
+
+          -- eapply binding_in_map_antimon.
+             2:{ eapply binding_in_map_set_lists; [| now eauto ].
+                 eapply binding_in_map_def_funs. eassumption. }
+             eapply occurs_free_in_fun. eapply find_def_correct. eassumption.
+
+    - intros x Hinx v Hgetx. destruct (Decidable_name_in_fundefs B).
+      destruct (Dec x).
+      + rewrite def_funs_eq in Hgetx; eauto. inv Hgetx.
+        edestruct name_in_fundefs_find_def_is_Some. eassumption. destructAll.
+        inv Hinx.
+
+        assert (Heq: L ! x = None).
+        { destruct (L ! x) eqn:Het; eauto. exfalso. eapply H1. eexists. eassumption. }
+        
+        edestruct Elim_fundefs_exists_None; try eassumption. eapply find_def_correct. eassumption.
+        destructAll. 
+
+        eexists. split.
+        * rewrite def_funs_eq. reflexivity.
+          eapply Elim_fundefs_name_in_fundefs with (B := B); eassumption. 
+
+        * rewrite preord_val_eq. intro; intros. repeat subst_exp.
+
+          edestruct (@set_lists_length3 val) with (xs := xs1) (vs := vs2) (rho := def_funs B' B' rho2 rho2).
+          rewrite <- H4. eapply set_lists_length_eq. now eauto.
+
+          assert (Hand : forall m, m < k ->
+                                   fun_inv L find_tag m (def_funs B B rho1 rho1) (def_funs B' B' rho2 rho2) /\
+                                   preord_env_P cenv PG
+                                                (name_in_fundefs B :|: occurs_free_fundefs B  \\ Dom_map L) m
+                                                (def_funs B B rho1 rho1) (def_funs B' B' rho2 rho2)).
+          { intros. eapply IHk; try eassumption.
+            - eapply fun_inv_monotonic. eassumption. omega.
+            - eapply preord_env_P_monotonic; [| eassumption ]. omega. } 
+          
+
+          do 3 eexists. repeat split.
+          -- eapply find_def_complete.
+             eapply unique_bindings_fundefs_unique_functions. 
+             eapply Elim_fundefs_unique_bindings. eassumption. eassumption.
+             eassumption. 
+          -- now eauto.
+          -- intros.
+             edestruct (Hand j) as [Hinv' Henv']. omega.
+
+             { eapply preord_exp_post_monotonic. eapply HGPost. eassumption.
+               eapply Elim_expr_correct with (S := Empty_set _); try eassumption. 
+               - eapply Disjoint_Included_r. eapply bound_var_occurs_free_in_fun_Included.
+                 eapply find_def_correct. eassumption. eassumption.
+               - eapply Dead_empty. eapply no_fun_in_fundefs. eassumption.
+                 eapply find_def_correct. eassumption.
+               - eapply Known_fundefs_fun_in_fundefs. eassumption. eapply find_def_correct. eassumption.                 
+               - assert (Hin : FromList xs1 \subset bound_var_fundefs B).
+                  { eapply Included_trans; [| eapply fun_in_fundefs_bound_var_fundefs; eapply find_def_correct; eassumption ].
+                    sets. } 
+                  eapply fun_inv_set_lists_Disjoint_l; eauto; sets.
+                  eapply fun_inv_set_lists_Disjoint_r; eauto; sets.
+               - normalize_sets.
+                 eapply preord_env_P_set_lists_l; eauto.
+
+                 intros. inv H10. eapply occurs_free_in_fun in H11; [| eapply find_def_correct; eassumption ].
+                 constructor; eauto. inv H11; eauto. exfalso; eauto.
+               - eapply binding_in_map_antimon. 
+                 2:{ eapply binding_in_map_set_lists; [| now eauto ].
+                     eapply binding_in_map_def_funs. eassumption. }
+                 eapply occurs_free_in_fun. eapply find_def_correct. eassumption. }
+
+      + rewrite def_funs_neq in Hgetx; eauto. rewrite def_funs_neq.
+        2:{ intros Hc. eapply n. eapply Elim_fundefs_name_in_fundefs in Hc; eauto. }
+        eapply Henv; eauto. inv Hinx. inv H; eauto.
+        now exfalso; eauto. constructor; eauto.
+  Qed.
+            
+         
+
+
+(*
+      
+Lemma eliminate_expr_correct: 
+  forall e sig fm st S
+         (Hun : unique_bindings e)          
+         (Hdis1 : Disjoint _ (Dom_map L) (bound_var e :|: occurs_free e))          
+         (Hnf : no_fun e)
+         
+         (Hd : Dead S L e)
+         (Hk : Known_exp (Dom_map L) e)
+         
+         (Hfinv : fun_inv F L rho1 rho2),
+    
+      {{ fun _ s => True }}
+        eliminate_expr L e 
+      {{ fun _ s e' s' =>
+           next_var (fst s) = next_var (fst s) /\
+           unique_bindings e' /\
+           occurs_free e' \subset occurs_free e /\
+           bound_var e' \subset bound_var e /\
+           (forall k rho1 rho2,
+               preord_env_P_inj cenv PG (occurs_free e \\ S \\ Dom_map L) k (apply_r sig) rho1 rho2 ->
+               binding_in_map (occurs_free e) ->                 
+               preord_exp cenv (P1 d) PG k (e, rho1) (e', rho2)) }}.
+
+    (forall B sig sig0 fm st S
+            (Hun : unique_bindings_fundefs B)
+            (Hdis1 : Disjoint _ (bound_var_fundefs B) (occurs_free_fundefs B :|: (occurs_free_fun_map fm \\ name_in_fundefs B)))
+            (Hdis3 : Disjoint _ S (image (apply_r sig) (occurs_free_fundefs B :|: occurs_free_fun_map fm)))
+            (Hdis4 : Disjoint _ (bound_var_fundefs B \\ name_in_fundefs B) (Dom_map fm))
+            (Hdis5 : just_for_fun_inv B fm)
+                        
+            (Hfm : fun_map_vars fm S sig)
+            (Hnames1 : NoDup (apply_r_list sig (all_fun_name B)))
+            (Hnames2 : Disjoint _ S (FromList (apply_r_list sig (all_fun_name B)))), 
+        {{ fun _ s => fresh S (next_var (fst s)) }}
+          inline_fundefs St IH d sig0 sig fm B st
+        {{ fun _ s B' s' =>
+             fresh S (next_var (fst s')) /\ next_var (fst s) <= next_var (fst s') /\
+             unique_bindings_fundefs B' /\
+             occurs_free_fundefs B' \subset image (apply_r sig) (occurs_free_fundefs B :|: occurs_free_fun_map fm) /\
+             bound_var_fundefs B' \\ name_in_fundefs B' \subset (Range (next_var (fst s)) (next_var (fst s'))) /\
+             all_fun_name B' = apply_r_list sig (all_fun_name B) /\
+             (forall f xs ft e1,
+                 find_def f B = Some (ft, xs, e1) ->
+                 exists xs' e2,
+                   find_def (apply_r sig f) B' = Some (ft, xs', e2) /\
+                   length xs = length xs' /\ NoDup xs' /\ FromList xs' \subset S /\
+                   (forall rho1 rho2 k,
+                       preord_env_P_inj cenv PG (occurs_free_fundefs B :|: name_in_fundefs B :|: FromList xs )
+                                        k (apply_r sig <{ xs ~> xs' }>) rho1 rho2 ->
+                       fun_map_inv d (occurs_free_fundefs B :|: name_in_fundefs B :|: FromList xs) fm rho1 rho2 k (set_list (combine xs xs') sig) ->
+                       preord_exp cenv (P1 d) PG k (e1, rho1) (e2, rho2))) }}).
+  
+  Proof.
+*)
